src/Std/Data/DTreeMap/Internal/Impl/Def.lean
@@ -32,12 +32,10 @@ inductive Impl (α : Type u) (β : α → Type v) where
   deriving Inhabited
 
 /-- The "delta" parameter of the size-bounded tree. Controls how imbalanced the tree can be. -/
-@[inline, tree_tac]
+@[inline]
 def delta : Nat := 3
 
 /-- The "ratio" parameter of the size-bounded tree. Controls how aggressive the rebalancing
 operations are. -/
-@[inline, tree_tac]
+@[inline]
 def ratio : Nat := 2
-
-macro "tree_simp₁" : tactic => `(tactic| simp only [delta, ratio])
